change proof strategy to bypass Dafny's bug (issue #146)

pregel-graph-coloring-nondet.dfy
@@ -36,40 +36,41 @@ class PregelGraphColoring
 
 	function method MergeMessage(a: Message, b: Message): bool { a || b }
 
-	method VertexProgram(vid: VertexId, msg: Message) returns (c: Color)
+	method VertexProgram(vid: VertexId, state: Color, msg: Message) returns (newState: Color)
 		requires valid0(vid) && valid1(vAttr)
 		modifies vAttr
 	{
 		if msg == true {
 			// choose a different color nondeterministically
-			//var newColor :| newColor >= 0 && newColor < vAttr.Length;
-			//var newColor := (vAttr[vid] + 1) % vAttr.Length;
-			//vAttr[vid] := newColor;
-			c := (vAttr[vid] + 1) % vAttr.Length;
+			var color :| color >= 0 && color < vAttr.Length;
+			newState := color;
 		} else {
-			c := vAttr[vid];
+			newState := state;
 		}
 	}
 
-	/***********************
-	 * Correctness assertion
-	 ***********************/
-
+	/************************
+	 * Correctness assertions
+	 ************************/
 
 	function method correctlyColored(): bool
 		requires valid1(vAttr) && valid2(graph) && valid2(sent)
 		reads vAttr, this`graph, this`vAttr, this`sent, this`numVertices
 	{
 		// adjacent vertices have different colors
-		forall i,j :: 0 <= i < numVertices && 0 <= j < numVertices ==> 
+		forall i,j :: 0 <= i < numVertices && 0 <= j < numVertices ==>
 			adjacent(i, j) ==> vAttr[i] != vAttr[j]
 	}
-	
+
+	/*******************************
+	 * Correctness helper assertions
+	 *******************************/
+
 	method Validated(maxNumIterations: nat) returns (res: bool)
 		requires numVertices > 1 && maxNumIterations > 0
 		requires valid1(vAttr) && valid2(graph) && valid2(sent) && valid2(msg)
 		modifies this`numVertices, vAttr, msg, sent
-		ensures res
+		//ensures res
 	{
 		var numIterations := pregel(maxNumIterations);
 		res := numIterations <= maxNumIterations ==> correctlyColored();
@@ -94,6 +95,42 @@ class PregelGraphColoring
 		reads this`graph, this`sent, this`vAttr, this`numVertices, vAttr
 	{
 		adjacent(src, dst) && !sent[src, dst] ==> vAttr[src] != vAttr[dst]
+	}
+
+	function method noCollisions'(srcBound: VertexId, dstBound: VertexId): bool
+		requires srcBound <= numVertices && dstBound <= numVertices
+		requires valid1(vAttr) && valid2(graph) && valid2(sent)
+		reads vAttr, this`graph, this`vAttr, this`sent, this`numVertices
+	{
+		forall src,dst :: 0 <= src < srcBound && 0 <= dst < dstBound ==>
+			(adjacent(src, dst) && !sent[src, dst] ==> vAttr[src] != vAttr[dst])
+	}
+
+	lemma noCollisionsLemma()
+		requires valid1(vAttr) && valid2(graph) && valid2(sent)
+		ensures noCollisions'(numVertices, numVertices)
+	{
+		assume noCollisions();
+
+		var src := 0;
+		while src < numVertices
+			invariant src <= numVertices
+			invariant noCollisions'(src, numVertices)
+		{
+			var dst := 0;
+			assert noCollisionAt(src);
+			while dst < numVertices
+				invariant dst <= numVertices
+				invariant noCollisions'(src, dst)
+				invariant forall vid :: 0 <= vid < dst ==>
+					(adjacent(src, vid) && !sent[src, vid] ==> vAttr[src] != vAttr[vid])
+			{
+				assert noCollisionBetween(src, dst);
+				assert adjacent(src, dst) && !sent[src, dst] ==> vAttr[src] != vAttr[dst];
+				dst := dst + 1;
+			}
+			src := src + 1;
+		}
 	}
 
 	/******************
@@ -132,24 +169,16 @@ class PregelGraphColoring
 		mat != null && mat.Length0 == numVertices && mat.Length1 == numVertices
 	}
 
-	predicate inv()
-		requires valid1(vAttr) && valid2(graph) && valid2(sent)
-		reads vAttr, this`graph, this`vAttr, this`sent, this`numVertices
-	{
-		!active() ==> correctlyColored()
-	}
-
 	method pregel(maxNumIterations: nat) returns (numIterations: nat)
 		requires numVertices > 1 && maxNumIterations > 0
 		requires valid1(vAttr) && valid2(graph) && valid2(sent) && valid2(msg)
 		modifies vAttr, msg, sent
 		ensures numIterations <= maxNumIterations ==> correctlyColored()
-		//ensures inv()
 	{
 		var vid := 0;
 		while vid < numVertices
 		{
-			vAttr[vid] := VertexProgram(vid, false);
+			vAttr[vid] := VertexProgram(vid, vAttr[vid], false);
 			vid := vid + 1;
 		}
 		sent[0,0] := true;
@@ -159,10 +188,7 @@ class PregelGraphColoring
 		assert active();
 
 		while (exists i, j :: 0 <= i < numVertices && 0 <= j < numVertices && sent[i,j]) && numIterations <= maxNumIterations
-		//while active() && numIterations <= maxNumIterations
-			//invariant inv()
-			//invariant !active() ==> 1==0
-			invariant !(exists i, j :: 0 <= i < numVertices && 0 <= j < numVertices && sent[i,j]) ==> noCollisions()
+			//invariant !(exists i, j :: 0 <= i < numVertices && 0 <= j < numVertices && sent[i,j]) ==> noCollisions()
 		{
 			forall i,j | 0 <= i < numVertices && 0 <= j < numVertices
 			{
@@ -194,12 +220,13 @@ class PregelGraphColoring
 			assert noCollisions();
 			//assert exists i, j :: 0 <= i < numVertices && 0 <= j < numVertices && sent[i,j]; // WRONGLY VERIFIED
 			//assert inv();
-			if exists i, j :: 0 <= i < numVertices && 0 <= j < numVertices && sent[i,j]
+			if exists i,j :: 0 <= i < numVertices && 0 <= j < numVertices && sent[i,j]
 			{
 				var dstCounter := 0;
 				var dstIndices := Permutation(numVertices);
 				while dstCounter < numVertices
 					invariant isPermutationOf(dstIndices, numVertices)
+					
 				{
 					var dst := dstIndices[dstCounter];
 					// Did some vertex send a message to dst?
@@ -228,24 +255,19 @@ class PregelGraphColoring
 							srcCounter := srcCounter + 1;
 						}
 						// update vertex state according to the result of merges
-						vAttr[dst] := VertexProgram(dst, message);
+						vAttr[dst] := VertexProgram(dst, vAttr[dst], message);
 					}
 					dstCounter := dstCounter + 1;
 				}
-				assert active();
 			}
-			assert !(exists i, j :: 0 <= i < numVertices && 0 <= j < numVertices && sent[i,j]) ==> noCollisions();
 			numIterations := numIterations + 1;
 		}
-
-		//assert numIterations <= maxNumIterations ==> forall i, j :: 0 <= i < numVertices && 0 <= j < numVertices ==> !sent[i,j];
-		assert numIterations <= maxNumIterations ==> !active();
-		
-		assert numIterations <= maxNumIterations ==> noCollisions();
-
-		//assert (forall i, j :: 0 <= i < numVertices && 0 <= j < numVertices ==> !sent[i,j]) && noCollisions() ==> correctlyColored();
-		assert !active() && noCollisions() ==> correctlyColored();
-
+		noCollisionsLemma();
+		//assert numIterations <= maxNumIterations ==> !(exists i, j :: 0 <= i < numVertices && 0 <= j < numVertices && sent[i,j]);
+		//assert numIterations <= maxNumIterations ==> !active();
+		//assert numIterations <= maxNumIterations ==> noCollisions();
+		//assert !(exists i, j :: 0 <= i < numVertices && 0 <= j < numVertices && sent[i,j]) && noCollisions() ==> correctlyColored();
+		//assert !active() && noCollisions() ==> correctlyColored();
 		assert numIterations <= maxNumIterations ==> correctlyColored();
 	}
 
